Working on stratification updates--not finished

Rewrites/ReflectionPre.v
@@ -932,7 +932,7 @@ Ltac KRExprReify e t :=
 
 Set Printing Implicit.
 
-Goal forall meth mdev, In meth (concat (map getAllMethods (map (fun m : RegFileBase => Base (BaseRegFile m)) mdev))).
+(*Goal forall meth mdev, In meth (concat (map getAllMethods (map (fun m : RegFileBase => Base (BaseRegFile m)) mdev))).
   intros.
   match goal with
   | |- ?X => let r := (ltac:(KRExprReify X (KRTypeElem KRElemProp))) in idtac r
@@ -940,7 +940,7 @@ Goal forall meth mdev, In meth (concat (map getAllMethods (map (fun m : RegFileB
   match goal with
   | |- In _ (concat (map getAllMethods ?X)) => let r := (ltac:(KRExprReify (map getAllMethods X) (KRTypeList (KRTypeList (KRTypeElem KRElemDefMethT))))) in idtac r
   end.
-Abort.
+Abort.*)
 
 Axiom cheat: forall x, x.
 
@@ -1877,110 +1877,76 @@ Definition KRSimplifyTop_list_Mod (e: KRExpr_list_Mod) : KRExpr_list_Mod :=
    | e => e
    end.
 
+(*********************************************************************************************************)
+
+Definition KRSimplify_RegInitValT (e : KRExpr_RegInitValT) : KRExpr_RegInitValT := KRSimplifyTop_RegInitValT e.
+
+Definition KRSimplify_ActionVoid(e : KRExpr_ActionVoid) : KRExpr_ActionVoid := KRSimplifyTop_ActionVoid e.
+
+Definition KRSimplify_MethodT(e: KRExpr_MethodT) : KRExpr_MethodT := KRSimplifyTop_MethodT e.
+
 Fixpoint KRSimplify_RegInitT (e : KRExpr_RegInitT) : KRExpr_RegInitT :=
   KRSimplifyTop_RegInitT (match e with
                           | KRPair_RegInitT f s => KRPair_RegInitT (KRSimplify_string f) (KRSimplify_RegInitValT s)
                           | _ => e
                           end)
                          
-with KRSimplify_RegInitValT (e : KRExpr_RegInitValT) : KRExpr_RegInitValT := KRSimplifyTop_RegInitValT e
+with KRSimplify_Rule (e : KRExpr_Rule) : KRExpr_Rule :=
+       KRSimplifyTop_Rule (match e with
+                           | KRPair_Rule f s => KRPair_Rule (KRSimplify_string f) (KRSimplify_ActionVoid s)
+                           | _ => e
+                          end)
 
-with KRSimplify_Rule (e : KRExpr_Rule) : KRExpr_Rule := KRSimplifyTop_Rule e
 
-with KRSimplify_DefMethT (e : KRExpr_DefMethT) : KRExpr_DefMethT := KRSimplifyTop_DefMethT e
+with KRSimplify_DefMethT (e : KRExpr_DefMethT) : KRExpr_DefMethT :=
+       KRSimplifyTop_DefMethT (match e with
+                               | KRPair_DefMethT f s => KRPair_DefMethT (KRSimplify_string f) (KRSimplify_MethodT s)
+                               | _ => e
+                               end)
 
-with KRSimplify_ModuleElt (e : KRExpr_ModuleElt) : KRExpr_ModuleElt :=
+with KRSimplify_string(s:KRExpr_string) :=
+       KRSimplifyTop_string (match s with
+                             | KRstring_append a b => KRstring_append (KRSimplify_string a) (KRSimplify_string b)
+                             | KRfst_RegInitT_string r => KRfst_RegInitT_string (KRSimplify_RegInitT r)
+                             | KRfst_DefMethT_string r => KRfst_DefMethT_string (KRSimplify_DefMethT r)
+                             | KRfst_Rule_string r => KRfst_Rule_string (KRSimplify_Rule r)
+                             | s => s
+                             end).
+
+
+Fixpoint KRSimplify_ModuleElt (e : KRExpr_ModuleElt) : KRExpr_ModuleElt :=
      KRSimplifyTop_ModuleElt (match e with
                               | KRMERegister r => KRMERegister (KRSimplify_RegInitT r)
                               | KRMERule r => KRMERule (KRSimplify_Rule r)
                               | KRMEMeth m => KRMEMeth (KRSimplify_DefMethT m)
                               | e => e
-                              end)
+                              end).
                              
-with KRSimplify_list_RegInitT (e : KRExpr_list_RegInitT) : KRExpr_list_RegInitT :=
-       KRSimplifyTop_list_RegInitT (match e with
-                                    | KRCons_list_RegInitT f r =>
-                                      KRCons_list_RegInitT (KRSimplify_RegInitT f) (KRSimplify_list_RegInitT r)
-                                    | KRApp_list_RegInitT f r =>
-                                      KRApp_list_RegInitT (KRSimplify_list_RegInitT f) (KRSimplify_list_RegInitT r)
-                                    | KRgetRegisters m => KRgetRegisters (KRSimplify_BaseModule m)
-                                    | KRgetAllRegisters m => KRgetAllRegisters (KRSimplify_Mod m)
-                                    | KRMakeModule_regs r => KRMakeModule_regs (KRSimplify_list_ModuleElt r)
-                                    | KRConcat_RegInitT r => KRConcat_RegInitT (KRSimplify_list_list_RegInitT r)
-                                    | e => e
-                                   end)
-  
-with KRSimplify_RegFileBase_list_RegInitT_Func (f: KRExpr_RegFileBase_list_RegInitT_Func) := f
+Definition KRSimplify_RegFileBase_Mod_Func(f: KRExpr_RegFileBase_Mod_Func) := f.
 
-with KRSimplify_list_list_RegInitT (e: KRExpr_list_list_RegInitT) : KRExpr_list_list_RegInitT :=
-       KRSimplifyTop_list_list_RegInitT (match e with
-                                         | KRCons_list_list_RegInitT f r =>
-                                           KRCons_list_list_RegInitT (KRSimplify_list_RegInitT f) (KRSimplify_list_list_RegInitT r)
-                                         | KRApp_list_list_RegInitT f r =>
-                                      KRApp_list_list_RegInitT (KRSimplify_list_list_RegInitT f) (KRSimplify_list_list_RegInitT r)
-                                         | KRMap_list_Mod_list_list_RegInitT f l => KRMap_list_Mod_list_list_RegInitT (KRSimplify_Mod_list_RegInitT_Func f) (KRSimplify_list_Mod l)
-                                         | KRMap_list_RegFileBase_list_list_RegInitT f l => KRMap_list_RegFileBase_list_list_RegInitT (KRSimplify_RegFileBase_list_RegInitT_Func f) (KRSimplify_list_RegFileBase l)
-                                         | e => e
-                                         end)
-  
-with KRSimplify_Mod_list_RegInitT_Func (f: KRExpr_Mod_list_RegInitT_Func) := f
+Definition KRSimplify_RegInitT_string_Func(f: KRExpr_RegInitT_string_Func) := f.
 
-with KRSimplify_list_Rule (e: KRExpr_list_Rule) : KRExpr_list_Rule :=
-       KRSimplifyTop_list_Rule (match e with
-                                | KRCons_list_Rule f r =>
-                                  KRCons_list_Rule (KRSimplify_Rule f) (KRSimplify_list_Rule r)
-                                | KRApp_list_Rule f r =>
-                                  KRApp_list_Rule (KRSimplify_list_Rule f) (KRSimplify_list_Rule r)
-                                | KRgetRules m => KRgetRules (KRSimplify_BaseModule m)
-                                | KRgetAllRules m => KRgetAllRules (KRSimplify_Mod m)
-                                | KRMakeModule_rules r => KRMakeModule_rules (KRSimplify_list_ModuleElt r)
-                                | KRConcat_Rule r => KRConcat_Rule (KRSimplify_list_list_Rule r)
-                                | e => e
-                               end)
+Definition KRSimplify_DefMethT_string_Func(f: KRExpr_DefMethT_string_Func) := f.
 
-with KRSimplify_Mod_list_Rule_Func(f: KRExpr_Mod_list_Rule_Func) := f
+Definition KRSimplify_Rule_string_Func(f: KRExpr_Rule_string_Func) := f.
 
-with KRSimplify_list_list_Rule (e: KRExpr_list_list_Rule) : KRExpr_list_list_Rule :=
-       KRSimplifyTop_list_list_Rule (match e with
-                                | KRCons_list_list_Rule f r =>
-                                  KRCons_list_list_Rule (KRSimplify_list_Rule f) (KRSimplify_list_list_Rule r)
-                                | KRApp_list_list_Rule f r =>
-                                  KRApp_list_list_Rule (KRSimplify_list_list_Rule f) (KRSimplify_list_list_Rule r)
-                                | KRMap_list_Mod_list_list_Rule f l =>  KRMap_list_Mod_list_list_Rule (KRSimplify_Mod_list_Rule_Func f) (KRSimplify_list_Mod l)
-                                | e => e
-                               end)
+Definition KRSimplify_Mod_Mod_PairFunc(f: KRExpr_Mod_Mod_PairFunc) := f.
 
-with KRSimplify_list_DefMethT (e: KRExpr_list_DefMethT) : KRExpr_list_DefMethT :=
-       KRSimplifyTop_list_DefMethT (match e with
-                                    | KRCons_list_DefMethT f r =>
-                                      KRCons_list_DefMethT (KRSimplify_DefMethT f) (KRSimplify_list_DefMethT r)
-                                    | KRApp_list_DefMethT f r =>
-                                      KRApp_list_DefMethT (KRSimplify_list_DefMethT f) (KRSimplify_list_DefMethT r)
-                                    | KRConcat_DefMethT r => KRConcat_DefMethT (KRSimplify_list_list_DefMethT r)
-                                    | KRgetMethods m => KRgetMethods (KRSimplify_BaseModule m)
-                                    | KRgetAllMethods m => KRgetAllMethods (KRSimplify_Mod m)
-                                    | KRMakeModule_meths r => KRMakeModule_meths (KRSimplify_list_ModuleElt r)
-                                    | e => e
-                                    end)
+Definition KRSimplify_Mod_list_DefMethT_Func(f: KRExpr_Mod_list_DefMethT_Func) := f.
 
-with KRSimplify_list_list_DefMethT (e: KRExpr_list_list_DefMethT) : KRExpr_list_list_DefMethT :=
-       KRSimplifyTop_list_list_DefMethT (match e with
-                                    | KRCons_list_list_DefMethT f r =>
-                                      KRCons_list_list_DefMethT (KRSimplify_list_DefMethT f) (KRSimplify_list_list_DefMethT r)
-                                    | KRApp_list_list_DefMethT f r =>
-                                      KRApp_list_list_DefMethT (KRSimplify_list_list_DefMethT f) (KRSimplify_list_list_DefMethT r)
-                                    | KRMap_list_Mod_list_list_DefMethT f l => KRMap_list_Mod_list_list_DefMethT (KRSimplify_Mod_list_DefMethT_Func f) (KRSimplify_list_Mod l)
-                                    | KRMap_list_RegFileBase_list_list_DefMethT f l => KRMap_list_RegFileBase_list_list_DefMethT (KRSimplify_RegFileBase_list_DefMethT_Func f) (KRSimplify_list_RegFileBase l)
-                                    | e => e
-                                    end)
+Definition KRSimplify_RegFileBase_list_DefMethT_Func(f: KRExpr_RegFileBase_list_DefMethT_Func) := f.
 
-with KRSimplify_Mod_list_DefMethT_Func(f: KRExpr_Mod_list_DefMethT_Func) := f
+Definition KRSimplify_RegFileBase_list_RegInitT_Func (f: KRExpr_RegFileBase_list_RegInitT_Func) := f.
 
-with KRSimplify_RegFileBase_list_DefMethT_Func(f: KRExpr_RegFileBase_list_DefMethT_Func) := f
+Definition KRSimplify_Mod_list_RegInitT_Func (f: KRExpr_Mod_list_RegInitT_Func) := f.
 
-with KRSimplify_CallWithSign(c: KRExpr_CallWithSign) := c
+Definition KRSimplify_Mod_list_Rule_Func(f: KRExpr_Mod_list_Rule_Func) := f.
 
-with KRSimplify_list_CallWithSign(e: KRExpr_list_CallWithSign) :=
+Definition KRSimplify_Mod_list_string_Func(f: KRExpr_Mod_list_string_Func) := f.
+
+Definition KRSimplify_CallWithSign(c: KRExpr_CallWithSign) := c.
+
+Fixpoint KRSimplify_list_CallWithSign(e: KRExpr_list_CallWithSign) :=
        KRSimplifyTop_list_CallWithSign (match e with
                                         | KRCons_list_CallWithSign f r =>
                                           KRCons_list_CallWithSign (KRSimplify_CallWithSign f) (KRSimplify_list_CallWithSign r)
@@ -1997,9 +1963,59 @@ with KRSimplify_list_list_CallWithSign(e: KRExpr_list_list_CallWithSign) :=
                                              | KRApp_list_list_CallWithSign f r =>
                                                KRApp_list_list_CallWithSign (KRSimplify_list_list_CallWithSign f) (KRSimplify_list_list_CallWithSign r)
                                              | e => e
-                                             end)
+                                             end).
 
-with KRSimplify_Mod_list_string_Func(f: KRExpr_Mod_list_string_Func) := f
+Definition KRSimplify_RegFileBase(m: KRExpr_RegFileBase) := m.
+
+Fixpoint KRSimplify_list_RegFileBase(e: KRExpr_list_RegFileBase) :=
+       KRSimplifyTop_list_RegFileBase (match e with
+                                      | KRCons_list_RegFileBase f r =>
+                                        KRCons_list_RegFileBase (KRSimplify_RegFileBase f) (KRSimplify_list_RegFileBase r)
+                                      | KRApp_list_RegFileBase f r =>
+                                        KRApp_list_RegFileBase (KRSimplify_list_RegFileBase f) (KRSimplify_list_RegFileBase r)
+                                      | e => e
+                                       end).
+
+Fixpoint KRSimplify_list_RegInitT (e : KRExpr_list_RegInitT) : KRExpr_list_RegInitT :=
+       KRSimplifyTop_list_RegInitT (match e with
+                                    | KRCons_list_RegInitT f r =>
+                                      KRCons_list_RegInitT (KRSimplify_RegInitT f) (KRSimplify_list_RegInitT r)
+                                    | KRApp_list_RegInitT f r =>
+                                      KRApp_list_RegInitT (KRSimplify_list_RegInitT f) (KRSimplify_list_RegInitT r)
+                                    | KRgetRegisters m => KRgetRegisters (KRSimplify_BaseModule m)
+                                    | KRgetAllRegisters m => KRgetAllRegisters (KRSimplify_Mod m)
+                                    | KRMakeModule_regs r => KRMakeModule_regs (KRSimplify_list_ModuleElt r)
+                                    | KRConcat_RegInitT r => KRConcat_RegInitT (KRSimplify_list_list_RegInitT r)
+                                    | e => e
+                                   end)
+with KRSimplify_list_list_RegInitT (e: KRExpr_list_list_RegInitT) : KRExpr_list_list_RegInitT :=
+       KRSimplifyTop_list_list_RegInitT (match e with
+                                         | KRCons_list_list_RegInitT f r =>
+                                           KRCons_list_list_RegInitT (KRSimplify_list_RegInitT f) (KRSimplify_list_list_RegInitT r)
+                                         | KRApp_list_list_RegInitT f r =>
+                                      KRApp_list_list_RegInitT (KRSimplify_list_list_RegInitT f) (KRSimplify_list_list_RegInitT r)
+                                         | KRMap_list_Mod_list_list_RegInitT f l => KRMap_list_Mod_list_list_RegInitT (KRSimplify_Mod_list_RegInitT_Func f) (KRSimplify_list_Mod l)
+                                         | KRMap_list_RegFileBase_list_list_RegInitT f l => KRMap_list_RegFileBase_list_list_RegInitT (KRSimplify_RegFileBase_list_RegInitT_Func f) (KRSimplify_list_RegFileBase l)
+                                         | e => e
+                                         end)
+
+with KRSimplify_BaseModule (e : KRExpr_BaseModule) : KRExpr_BaseModule :=
+       KRSimplifyTop_BaseModule
+         (match e with
+          | KRMakeModule e => KRMakeModule (KRSimplify_list_ModuleElt e)
+          | KRBaseMod regs rules meths => KRBaseMod (KRSimplify_list_RegInitT regs) (KRSimplify_list_Rule rules) (KRSimplify_list_DefMethT meths)
+          | KRBaseRegFile b => KRBaseRegFile (KRSimplify_RegFileBase b)
+          | e => e
+          end)
+
+with KRSimplify_Mod (e : KRExpr_Mod) : KRExpr_Mod :=
+       KRSimplifyTop_Mod
+         (match e with
+          | KRBase b => KRBase (KRSimplify_BaseModule b)
+          | KRConcatMod a b => KRConcatMod (KRSimplify_Mod a) (KRSimplify_Mod b)
+          | KRFold_right_Mod f a b => KRFold_right_Mod (KRSimplify_Mod_Mod_PairFunc f) (KRSimplify_Mod a) (KRSimplify_list_Mod b)
+          | e => e
+          end)
 
 with KRSimplify_list_ModuleElt (e: KRExpr_list_ModuleElt) : KRExpr_list_ModuleElt :=
        KRSimplifyTop_list_ModuleElt (match e with
@@ -2013,46 +2029,6 @@ with KRSimplify_list_ModuleElt (e: KRExpr_list_ModuleElt) : KRExpr_list_ModuleEl
                                       | e => e
                                      end)
 
-with KRSimplify_list_list_ModuleElt (e: KRExpr_list_list_ModuleElt) : KRExpr_list_list_ModuleElt :=
-       KRSimplifyTop_list_list_ModuleElt (match e with
-                                      | KRCons_list_list_ModuleElt f r =>
-                                        KRCons_list_list_ModuleElt (KRSimplify_list_ModuleElt f) (KRSimplify_list_list_ModuleElt r)
-                                      | KRApp_list_list_ModuleElt f r =>
-                                        KRApp_list_list_ModuleElt (KRSimplify_list_list_ModuleElt f) (KRSimplify_list_list_ModuleElt r)
-                                      | e => e
-                                     end)
-
-with KRSimplify_BaseModule (e : KRExpr_BaseModule) : KRExpr_BaseModule :=
-       KRSimplifyTop_BaseModule
-         (match e with
-          | KRMakeModule e => KRMakeModule (KRSimplify_list_ModuleElt e)
-          | KRBaseMod regs rules meths => KRBaseMod (KRSimplify_list_RegInitT regs) (KRSimplify_list_Rule rules) (KRSimplify_list_DefMethT meths)
-          | KRBaseRegFile b => KRBaseRegFile (KRSimplify_RegFileBase b)
-          | e => e
-          end)
-
-with KRSimplify_RegFileBase(m: KRExpr_RegFileBase) := m
-    
-with KRSimplify_list_RegFileBase(e: KRExpr_list_RegFileBase) :=
-       KRSimplifyTop_list_RegFileBase (match e with
-                                      | KRCons_list_RegFileBase f r =>
-                                        KRCons_list_RegFileBase (KRSimplify_RegFileBase f) (KRSimplify_list_RegFileBase r)
-                                      | KRApp_list_RegFileBase f r =>
-                                        KRApp_list_RegFileBase (KRSimplify_list_RegFileBase f) (KRSimplify_list_RegFileBase r)
-                                      | e => e
-                                     end)
- 
-with KRSimplify_Mod (e : KRExpr_Mod) : KRExpr_Mod :=
-       KRSimplifyTop_Mod
-         (match e with
-          | KRBase b => KRBase (KRSimplify_BaseModule b)
-          | KRConcatMod a b => KRConcatMod (KRSimplify_Mod a) (KRSimplify_Mod b)
-          | KRFold_right_Mod f a b => KRFold_right_Mod (KRSimplify_Mod_Mod_PairFunc f) (KRSimplify_Mod a) (KRSimplify_list_Mod b)
-          | e => e
-          end)
-         
-with KRSimplify_Mod_Mod_PairFunc(f: KRExpr_Mod_Mod_PairFunc) := f
-
 with KRSimplify_list_Mod(e: KRExpr_list_Mod) :=
        KRSimplifyTop_list_Mod (match e with
                                | KRCons_list_Mod f r =>
@@ -2062,24 +2038,63 @@ with KRSimplify_list_Mod(e: KRExpr_list_Mod) :=
                                | e => e
                                end)
 
-with KRSimplify_RegFileBase_Mod_Func(f: KRExpr_RegFileBase_Mod_Func) := f
+with KRSimplify_list_DefMethT (e: KRExpr_list_DefMethT) : KRExpr_list_DefMethT :=
+       KRSimplifyTop_list_DefMethT (match e with
+                                    | KRCons_list_DefMethT f r =>
+                                      KRCons_list_DefMethT (KRSimplify_DefMethT f) (KRSimplify_list_DefMethT r)
+                                    | KRApp_list_DefMethT f r =>
+                                      KRApp_list_DefMethT (KRSimplify_list_DefMethT f) (KRSimplify_list_DefMethT r)
+                                    | KRConcat_DefMethT r => KRConcat_DefMethT (KRSimplify_list_list_DefMethT r)
+                                    | KRgetMethods m => KRgetMethods (KRSimplify_BaseModule m)
+                                    | KRgetAllMethods m => KRgetAllMethods (KRSimplify_Mod m)
+                                    | KRMakeModule_meths r => KRMakeModule_meths (KRSimplify_list_ModuleElt r)
+                                    | e => e
+                                    end)
 
-with KRSimplify_RegInitT_string_Func(f: KRExpr_RegInitT_string_Func) := f
+with KRSimplify_list_Rule (e: KRExpr_list_Rule) : KRExpr_list_Rule :=
+       KRSimplifyTop_list_Rule (match e with
+                                | KRCons_list_Rule f r =>
+                                  KRCons_list_Rule (KRSimplify_Rule f) (KRSimplify_list_Rule r)
+                                | KRApp_list_Rule f r =>
+                                  KRApp_list_Rule (KRSimplify_list_Rule f) (KRSimplify_list_Rule r)
+                                | KRgetRules m => KRgetRules (KRSimplify_BaseModule m)
+                                | KRgetAllRules m => KRgetAllRules (KRSimplify_Mod m)
+                                | KRMakeModule_rules r => KRMakeModule_rules (KRSimplify_list_ModuleElt r)
+                                | KRConcat_Rule r => KRConcat_Rule (KRSimplify_list_list_Rule r)
+                                | e => e
+                               end)
 
-with KRSimplify_DefMethT_string_Func(f: KRExpr_DefMethT_string_Func) := f
+with KRSimplify_list_list_Rule (e: KRExpr_list_list_Rule) : KRExpr_list_list_Rule :=
+       KRSimplifyTop_list_list_Rule (match e with
+                                | KRCons_list_list_Rule f r =>
+                                  KRCons_list_list_Rule (KRSimplify_list_Rule f) (KRSimplify_list_list_Rule r)
+                                | KRApp_list_list_Rule f r =>
+                                  KRApp_list_list_Rule (KRSimplify_list_list_Rule f) (KRSimplify_list_list_Rule r)
+                                | KRMap_list_Mod_list_list_Rule f l =>  KRMap_list_Mod_list_list_Rule (KRSimplify_Mod_list_Rule_Func f) (KRSimplify_list_Mod l)
+                                | e => e
+                               end)
 
-with KRSimplify_Rule_string_Func(f: KRExpr_Rule_string_Func) := f
+with KRSimplify_list_list_DefMethT (e: KRExpr_list_list_DefMethT) : KRExpr_list_list_DefMethT :=
+       KRSimplifyTop_list_list_DefMethT (match e with
+                                    | KRCons_list_list_DefMethT f r =>
+                                      KRCons_list_list_DefMethT (KRSimplify_list_DefMethT f) (KRSimplify_list_list_DefMethT r)
+                                    | KRApp_list_list_DefMethT f r =>
+                                      KRApp_list_list_DefMethT (KRSimplify_list_list_DefMethT f) (KRSimplify_list_list_DefMethT r)
+                                    | KRMap_list_Mod_list_list_DefMethT f l => KRMap_list_Mod_list_list_DefMethT (KRSimplify_Mod_list_DefMethT_Func f) (KRSimplify_list_Mod l)
+                                    | KRMap_list_RegFileBase_list_list_DefMethT f l => KRMap_list_RegFileBase_list_list_DefMethT (KRSimplify_RegFileBase_list_DefMethT_Func f) (KRSimplify_list_RegFileBase l)
+                                    | e => e
+                                    end).
 
-with KRSimplify_string(s:KRExpr_string) :=
-       KRSimplifyTop_string (match s with
-                             | KRstring_append a b => KRstring_append (KRSimplify_string a) (KRSimplify_string b)
-                             | KRfst_RegInitT_string r => KRfst_RegInitT_string (KRSimplify_RegInitT r)
-                             | KRfst_DefMethT_string r => KRfst_DefMethT_string (KRSimplify_DefMethT r)
-                             | KRfst_Rule_string r => KRfst_Rule_string (KRSimplify_Rule r)
-                             | s => s
-                             end)
+Fixpoint KRSimplify_list_list_ModuleElt (e: KRExpr_list_list_ModuleElt) : KRExpr_list_list_ModuleElt :=
+       KRSimplifyTop_list_list_ModuleElt (match e with
+                                      | KRCons_list_list_ModuleElt f r =>
+                                        KRCons_list_list_ModuleElt (KRSimplify_list_ModuleElt f) (KRSimplify_list_list_ModuleElt r)
+                                      | KRApp_list_list_ModuleElt f r =>
+                                        KRApp_list_list_ModuleElt (KRSimplify_list_list_ModuleElt f) (KRSimplify_list_list_ModuleElt r)
+                                      | e => e
+                                     end).
 
-with KRSimplify_list_string(e: KRExpr_list_string) :=
+Fixpoint KRSimplify_list_string(e: KRExpr_list_string) :=
        KRSimplifyTop_list_string (match e with
                                | KRCons_list_string f r =>
                                  KRCons_list_string (KRSimplify_string f) (KRSimplify_list_string r)
@@ -2100,9 +2115,9 @@ with KRSimplify_list_list_string(e: KRExpr_list_list_string) :=
                                        | KRApp_list_list_string f r =>
                                          KRApp_list_list_string (KRSimplify_list_list_string f) (KRSimplify_list_list_string r)
                                        | e => e
-                                       end)
+                                       end).
 
-with KRSimplify_Prop(p:KRExpr_Prop) :=
+Fixpoint KRSimplify_Prop(p:KRExpr_Prop) :=
        KRSimplifyTop_Prop (match p with
                            | KRAnd_Prop a b => KRAnd_Prop (KRSimplify_Prop a) (KRSimplify_Prop b)
                            | KROr_Prop a b => KROr_Prop (KRSimplify_Prop a) (KRSimplify_Prop b)
@@ -2121,6 +2136,7 @@ with KRSimplify_Prop(p:KRExpr_Prop) :=
                            | p => p
                            end).
 
+(*********************************************************************************************************)
 
 Ltac match_KRExprType t :=
   match t with
@@ -2128,6 +2144,8 @@ Ltac match_KRExprType t :=
   | KRExpr_list_RegInitT => idtac
   | KRExpr_list_list_RegInitT => idtac
   | KRExpr_RegInitValT => idtac
+  | KRExpr_DefMethT => idtac
+  | KRExpr_ActionVoid => idtac
   | KRExpr_Rule => idtac
   | KRExpr_list_Rule => idtac
   | KRExpr_list_list_Rule => idtac
@@ -2145,12 +2163,17 @@ Ltac match_KRExprType t :=
   | KRExpr_list_Mod => idtac
   | KRExpr_RegFileBase => idtac
   | KRExpr_list_RegFileBase => idtac
+  | KRExpr_string => idtac
+  | KRExpr_list_string => idtac
+  | KRExpr_list_list_string => idtac
   end.
 
 Ltac match_KRExprDenote d :=
   match d with
   | KRExprDenote_RegInitT => idtac
   | KRExprDenote_RegInitValT => idtac
+  | KRExprDenote_DefMethT => idtac
+  | KRExprDenote_ActionVoid => idtac
   | KRExprDenote_list_RegInitT => idtac
   | KRExprDenote_list_list_RegInitT => idtac
   | KRExprDenote_Rule => idtac
@@ -2170,6 +2193,9 @@ Ltac match_KRExprDenote d :=
   | KRExprDenote_list_Mod => idtac
   | KRExprDenote_RegFileBase => idtac
   | KRExprDenote_list_RegFileBase => idtac
+  | KRExprDenote_string => idtac
+  | KRExprDenote_list_string => idtac
+  | KRExprDenote_list_list_string => idtac
   end.
 
 Ltac isVar x :=
@@ -2183,7 +2209,9 @@ Ltac step_KRSimplifyTopSound :=
   | _ => progress intros
   | _ => progress simpl
   | _ => progress (autorewrite with kami_rewrite_db)
+  | _ => progress (autorewrite with KRSimplify)
   | _ => progress reflexivity
+  | |- (_,_)=(_,_) => progress f_equal
   end.
 
 Ltac solve_contKRSimplifyTopSound :=
@@ -2354,12 +2382,13 @@ KRExpr_list_ModuleElt_mut, KRExpr_list_list_ModuleElt_mut, KRExpr_BaseModule_mut
 
 Ltac noDenote x :=
   match x with
-  | context [ ?D _ ] => match_KRExprDenote ?D;fail 1
+  | context [ ?D _ ] => match_KRExprDenote D;fail 1
   | _ => idtac
   end.
 
 Ltac KRSimplifySound_unit :=
   match goal with
+  | |- (_,_)=(_,_) => f_equal
   | _ => reflexivity
   | _ => progress simpl
   (*| |- _ = KRExprDenote_Mod (match KRSimplify_Mod ?V with
@@ -2373,28 +2402,55 @@ Ltac KRSimplifySound_unit :=
   | H: KRVar_RegInitT_string_Func _ =  KRVar_RegInitT_string_Func _ |- _ => inversion H;subst;clear H
   | _ => progress subst
   | _ => progress (autorewrite with kami_rewrite_db)
+  | _ => progress (autorewrite with KRSimplify)
   | H: KRExprDenote_BaseModule _ = ?R |- _ => noDenote R;rewrite H
-  | H: KRExprDenote_string _ = _ |- ?R => noDenote R;rewrite H
-  | H: KRExprDenote_list_string _ = _ |- ?R => noDenote R;rewrite H
-  | H: KRExprDenote_list_list_string _ = _ |- ?R => noDenote R;rewrite H
-  | H: KRExprDenote_Mod _ = _ |- ?R => noDenote R;rewrite H
+  | H: KRExprDenote_string _ = ?R |- _ => noDenote R;rewrite H
+  | H: KRExprDenote_list_string _ = ?R |- _ => noDenote R;rewrite H
+  | H: KRExprDenote_list_list_string _ = ?R |- _ => noDenote R;rewrite H
+  | H: KRExprDenote_Mod _ = ?R |- _ => noDenote R;rewrite H
   | H: KRExprDenote_list_Mod _ = ?R |- _ => noDenote R;rewrite H
   | H: KRExprDenote_RegInitT _ = ?R |- _ => noDenote R;rewrite H
   | H: KRExprDenote_RegInitValT _ = ?R |- _ => noDenote R;rewrite H
+  | H: KRExprDenote_DefMethT _ = ?R |- _ => noDenote R;rewrite H
+  | H: KRExprDenote_ActionVoid _ = ?R |- _ => noDenote R;rewrite H
   | H: KRExprDenote_list_RegInitT _ = ?R |- _ => noDenote R;rewrite H
   | H: KRExprDenote_list_list_RegInitT _ = ?R |- _ => noDenote R;rewrite H
-  | H: KRExprDenote_Rule _ = _ |- ?R => noDenote R;rewrite H
-  | H: KRExprDenote_list_Rule _ = _ |- ?R => noDenote R;rewrite H
-  | H: KRExprDenote_list_list_Rule _ = _ |- ?R => noDenote R;rewrite H
-  | H: KRExprDenote_DefMethT _ = _ |- ?R => noDenote R;rewrite H
-  | H: KRExprDenote_list_DefMethT _ = _ |- ?R => noDenote R;rewrite H
+  | H: KRExprDenote_Rule _ = ?R |- _ => noDenote R;rewrite H
+  | H: KRExprDenote_list_Rule _ = ?R |- _ => noDenote R;rewrite H
+  | H: KRExprDenote_list_list_Rule _ = ?R |- _ => noDenote R;rewrite H
+  | H: KRExprDenote_DefMethT _ = ?R |- _ => noDenote R;rewrite H
+  | H: KRExprDenote_list_DefMethT _ = ?R |- _ => noDenote R;rewrite H
   | H: KRExprDenote_list_list_DefMethT _ = ?R |- _ => noDenote R;rewrite H
-  | H: KRExprDenote_RegFileBase _ = _ |- ?R => noDenote R;rewrite H
-  | H: KRExprDenote_list_RegFileBase _ = _ |- ?R => noDenote R;rewrite H
-  | H: KRExprDenote_CallWithSign _ = _ |- ?R => noDenote R;rewrite H
-  | H: KRExprDenote_list_CallWithSign _ = _ |- ?R => noDenote R;rewrite H
+  | H: KRExprDenote_RegFileBase _ = ?R |- _ => noDenote R;rewrite H
+  | H: KRExprDenote_list_RegFileBase _ = ?R |- _ => noDenote R;rewrite H
+  | H: KRExprDenote_CallWithSign _ = ?R |- _ => noDenote R;rewrite H
+  | H: KRExprDenote_list_CallWithSign _ = ?R |- _ => noDenote R;rewrite H
   | H: KRExprDenote_list_list_CallWithSign _ = ?R |- _ => noDenote R;rewrite H
-  | H: KRExprDenote_Prop _ = _ |- ?R => noDenote R;rewrite H
+  | H: KRExprDenote_Prop _ = ?R |- _ => noDenote R;rewrite H
+  | H: ?R = KRExprDenote_BaseModule _ |- _ => noDenote R;rewrite <- H
+  | H: ?R = KRExprDenote_string _ |- _ => noDenote R;rewrite <- H
+  | H: ?R = KRExprDenote_list_string _ |- _ => noDenote R;rewrite H
+  | H: ?R = KRExprDenote_list_list_string _ |- _ => noDenote R;rewrite H
+  | H: ?R = KRExprDenote_Mod _ |- _ => noDenote R;rewrite H
+  | H: ?R = KRExprDenote_list_Mod _ |- _ => noDenote R;rewrite H
+  | H: ?R = KRExprDenote_RegInitT _ |- _ => noDenote R;rewrite H
+  | H: ?R = KRExprDenote_RegInitValT _ |- _ => noDenote R;rewrite H
+  | H: ?R = KRExprDenote_DefMethT _ |- _ => noDenote R;rewrite H
+  | H: ?R = KRExprDenote_ActionVoid _ |- _ => noDenote R;rewrite H
+  | H: ?R = KRExprDenote_list_RegInitT _ |- _ => noDenote R;rewrite H
+  | H: ?R = KRExprDenote_list_list_RegInitT _ |- _ => noDenote R;rewrite H
+  | H: ?R = KRExprDenote_Rule _ |- _ => noDenote R;rewrite H
+  | H: ?R = KRExprDenote_list_Rule _ |- _ => noDenote R;rewrite H
+  | H: ?R = KRExprDenote_list_list_Rule _ |- _ => noDenote R;rewrite H
+  | H: ?R = KRExprDenote_DefMethT _ |- _ => noDenote R;rewrite H
+  | H: ?R = KRExprDenote_list_DefMethT _ |- _ => noDenote R;rewrite H
+  | H: ?R = KRExprDenote_list_list_DefMethT _ |- _ => noDenote R;rewrite H
+  | H: ?R = KRExprDenote_RegFileBase _ |- _ => noDenote R;rewrite H
+  | H: ?R = KRExprDenote_list_RegFileBase _ |- _ => noDenote R;rewrite H
+  | H: ?R = KRExprDenote_CallWithSign _ |- _ => noDenote R;rewrite H
+  | H: ?R = KRExprDenote_list_CallWithSign _ |- _ => noDenote R;rewrite H
+  | H: ?R = KRExprDenote_list_list_CallWithSign _ |- _ => noDenote R;rewrite H
+  | H: ?R = KRExprDenote_Prop _ |- _ => noDenote R;rewrite H
   | H: _ = True |- _ => rewrite H
   | H: _ = False |- _ => rewrite H
   | H: True = _ |- _ => rewrite <- H
@@ -2488,9 +2544,119 @@ Ltac KRSimplifySound_crunch :=
 
 Theorem KRSimplify_RegInitValT_trivial:
   forall x, (KRSimplify_RegInitValT x)=x.
-Admitted.
+Proof.
+  reflexivity.
+Qed.
 
-Hint Rewrite KRSimplify_RegInitValT_trivial : kami_rewrite_db.
+Hint Rewrite KRSimplify_RegInitValT_trivial : KRSimplify.
+
+Theorem KRSimplify_MethodT_trivial:
+  forall x, (KRSimplify_MethodT x)=x.
+Proof.
+  reflexivity.
+Qed.
+
+Hint Rewrite KRSimplify_MethodT_trivial : KRSimplify.
+
+Theorem KRSimplify_ActionVoid_trivial:
+  forall x, (KRSimplify_ActionVoid x)=x.
+Proof.
+  reflexivity.
+Qed.
+
+Hint Rewrite KRSimplify_ActionVoid_trivial : KRSimplify.
+
+Theorem KRSimplify_RegFileBase_trivial:
+  forall x, (KRSimplify_RegFileBase x)=x.
+Proof.
+  reflexivity.
+Qed.
+
+Hint Rewrite KRSimplify_RegFileBase_trivial : KRSimplify.
+
+Theorem KRSimplify_RegFileBase_Mod_Func_trivial: forall x, KRSimplify_RegFileBase_Mod_Func x = x.
+Proof.
+  reflexivity.
+Qed.
+
+Hint Rewrite KRSimplify_RegFileBase_Mod_Func_trivial : KRSimplify.
+
+Theorem KRSimplify_RegInitT_string_Func_trivial: forall f, KRSimplify_RegInitT_string_Func f = f.
+Proof.
+  reflexivity.
+Qed.
+
+Hint Rewrite KRSimplify_RegInitT_string_Func_trivial : KRSimplify.
+
+Theorem KRSimplify_DefMethT_string_Func_trivial: forall f, KRSimplify_DefMethT_string_Func f=f.
+Proof.
+  reflexivity.
+Qed.
+
+Hint Rewrite KRSimplify_DefMethT_string_Func_trivial : KRSimplify.
+
+Theorem KRSimplify_Rule_string_Func_trivial: forall f, KRSimplify_Rule_string_Func f=f.
+Proof.
+  reflexivity.
+Qed.
+
+Hint Rewrite KRSimplify_Rule_string_Func_trivial : KRSimplify.
+
+Theorem KRSimplify_Mod_Mod_PairFunc_trivial: forall f, KRSimplify_Mod_Mod_PairFunc f = f.
+Proof.
+  reflexivity.
+Qed.
+
+Hint Rewrite KRSimplify_Mod_Mod_PairFunc_trivial : KRSimplify.
+
+Theorem KRSimplify_Mod_list_DefMethT_Func_trivial: forall f, KRSimplify_Mod_list_DefMethT_Func f = f.
+Proof.
+  reflexivity.
+Qed.
+
+Hint Rewrite KRSimplify_Mod_list_DefMethT_Func_trivial : KRSimplify.
+
+Theorem KRSimplify_RegFileBase_list_DefMethT_Func_trivial: forall f, KRSimplify_RegFileBase_list_DefMethT_Func f = f.
+Proof.
+  reflexivity.
+Qed.
+
+Hint Rewrite KRSimplify_RegFileBase_list_DefMethT_Func_trivial : KRSimplify.
+
+Theorem KRSimplify_RegFileBase_list_RegInitT_Func_trivial: forall f, KRSimplify_RegFileBase_list_RegInitT_Func f = f.
+Proof.
+  reflexivity.
+Qed.
+
+Hint Rewrite KRSimplify_RegFileBase_list_RegInitT_Func_trivial : KRSimplify.
+
+Theorem KRSimplify_Mod_list_RegInitT_Func_trivial: forall f, KRSimplify_Mod_list_RegInitT_Func f = f.
+Proof.
+  reflexivity.
+Qed.
+
+Hint Rewrite KRSimplify_Mod_list_RegInitT_Func_trivial : KRSimplify.
+
+Theorem KRSimplify_Mod_list_Rule_Func_trivial: forall f, KRSimplify_Mod_list_Rule_Func f = f.
+Proof.
+  reflexivity.
+Qed.
+
+Hint Rewrite KRSimplify_Mod_list_Rule_Func_trivial : KRSimplify.
+
+Theorem KRSimplify_Mod_list_string_Func_trivial: forall f, KRSimplify_Mod_list_string_Func f = f.
+Proof.
+  reflexivity.
+Qed.
+
+Hint Rewrite KRSimplify_Mod_list_string_Func_trivial : KRSimplify.
+
+Theorem KRSimplify_CallWithSign_trivial: forall c, KRSimplify_CallWithSign c = c.
+Proof.
+  reflexivity.
+Qed.
+
+Hint Rewrite KRSimplify_CallWithSign_trivial : KRSimplify.
 
 Theorem KRSimplify_list_RegInitT_KRApp_list_RegInitT : forall k k0,
     KRSimplify_list_RegInitT (KRApp_list_RegInitT k k0)=KRSimplifyTop_list_RegInitT (KRApp_list_RegInitT (KRSimplify_list_RegInitT k) (KRSimplify_list_RegInitT k0)).
