Rewrites/ReflectionSoundTheorems2.v
@@ -5,133 +5,30 @@ Require Import Kami.Notations_rewrites.
 Require Import Program.Equality.
 Require Import Kami.Rewrites.ReflectionPre.
 Require Import Kami.Rewrites.ReflectionSoundTopTheorems.
+Require Import Kami.Rewrites.ReflectionSoundTheorems1.
 
-Theorem KRSimplifySound_list_list_Rule: forall e,
-    KRExprDenote_list_list_Rule e = KRExprDenote_list_list_Rule (KRSimplify_list_list_Rule e).
-Proof.
-  KRSimplifySound_setup KRExpr_list_list_Rule_mut H H0 H1.
-  repeat KRSimplifySound_unit.
-  repeat KRSimplifySound_crunch.
-  - repeat KRSimplifySound_crunch.
-  - repeat KRSimplifySound_crunch.
-  - repeat KRSimplifySound_crunch.
-  - repeat KRSimplifySound_crunch.
-  - repeat KRSimplifySound_crunch.
-  - repeat KRSimplifySound_crunch.
-  - repeat KRSimplifySound_crunch.
-  - repeat KRSimplifySound_crunch.
-  - repeat KRSimplifySound_crunch.
-  - repeat KRSimplifySound_crunch.
-  - repeat KRSimplifySound_crunch.
-  - repeat KRSimplifySound_crunch.
-  - repeat KRSimplifySound_crunch.
-  - repeat KRSimplifySound_crunch.
-  - repeat KRSimplifySound_crunch.
-  - repeat KRSimplifySound_crunch.
-  - repeat KRSimplifySound_crunch.
-  - repeat KRSimplifySound_crunch.
-  - repeat KRSimplifySound_crunch.
-  - repeat KRSimplifySound_crunch.
-  - repeat KRSimplifySound_crunch.
-  - repeat KRSimplifySound_crunch.
-  - repeat KRSimplifySound_crunch.
-  - repeat KRSimplifySound_crunch.
-  - repeat KRSimplifySound_crunch.
-  - repeat KRSimplifySound_crunch.
-  - repeat KRSimplifySound_crunch.
-  - repeat KRSimplifySound_crunch.
-  - repeat KRSimplifySound_crunch.
-  - repeat KRSimplifySound_crunch.
-    replace (KRExprDenote_string k1 = KRExprDenote_string (KRSimplify_string k)) with
-        (KRExprDenote_string (KRSimplify_string k) = KRExprDenote_string k1). reflexivity.
-    apply my_eq_refl.
-  - repeat KRSimplifySound_crunch.
-    erewrite sdisjPrefix_false.
-    + reflexivity.
-    + rewrite HeqH2.
-      reflexivity.
-  - repeat KRSimplifySound_crunch.
-    replace (KRExprDenote_RegInitT k1 = KRExprDenote_RegInitT (KRSimplify_RegInitT k)) with
-        (KRExprDenote_RegInitT (KRSimplify_RegInitT k) = KRExprDenote_RegInitT k1). reflexivity.
-    apply my_eq_refl.
-  - repeat KRSimplifySound_crunch.
-    replace (KRExprDenote_Rule k1 = KRExprDenote_Rule (KRSimplify_Rule k)) with
-        (KRExprDenote_Rule (KRSimplify_Rule k) = KRExprDenote_Rule k1). reflexivity.
-    apply my_eq_refl.
-  - repeat KRSimplifySound_crunch.
-    replace (KRExprDenote_DefMethT k1 = KRExprDenote_DefMethT (KRSimplify_DefMethT k)) with
-        (KRExprDenote_DefMethT (KRSimplify_DefMethT k) = KRExprDenote_DefMethT k1). reflexivity.
-    apply my_eq_refl.
-  - repeat KRSimplifySound_crunch.
-  - repeat KRSimplifySound_crunch.
-  - repeat KRSimplifySound_crunch.
-Qed.
-  
-Theorem KRSimplifySound_list_list_DefMethT: forall e,
-    KRExprDenote_list_list_DefMethT e = KRExprDenote_list_list_DefMethT (KRSimplify_list_list_DefMethT e).
-Proof.
-  KRSimplifySound_setup KRExpr_list_list_DefMethT_mut H H0 H1.
-  repeat KRSimplifySound_unit.
-  repeat KRSimplifySound_crunch.
-  - repeat KRSimplifySound_crunch.
-  - repeat KRSimplifySound_crunch.
-  - repeat KRSimplifySound_crunch.
-  - repeat KRSimplifySound_crunch.
-  - repeat KRSimplifySound_crunch.
-  - repeat KRSimplifySound_crunch.
-  - repeat KRSimplifySound_crunch.
-  - repeat KRSimplifySound_crunch.
-  - repeat KRSimplifySound_crunch.
-  - repeat KRSimplifySound_crunch.
-  - repeat KRSimplifySound_crunch.
-  - repeat KRSimplifySound_crunch.
-  - repeat KRSimplifySound_crunch.
-  - repeat KRSimplifySound_crunch.
-  - repeat KRSimplifySound_crunch.
-  - repeat KRSimplifySound_crunch.
-  - repeat KRSimplifySound_crunch.
-  - repeat KRSimplifySound_crunch.
-  - repeat KRSimplifySound_crunch.
-  - repeat KRSimplifySound_crunch.
-  - repeat KRSimplifySound_crunch.
-  - repeat KRSimplifySound_crunch.
-  - repeat KRSimplifySound_crunch.
-  - repeat KRSimplifySound_crunch.
-  - repeat KRSimplifySound_crunch.
-  - repeat KRSimplifySound_crunch.
-  - repeat KRSimplifySound_crunch.
-  - repeat KRSimplifySound_crunch.
-  - repeat KRSimplifySound_crunch.
-  - repeat KRSimplifySound_crunch.
-    replace (KRExprDenote_string k1 = KRExprDenote_string (KRSimplify_string k)) with
-        (KRExprDenote_string (KRSimplify_string k) = KRExprDenote_string k1). reflexivity.
-    apply my_eq_refl.
-  - repeat KRSimplifySound_crunch.
-    erewrite sdisjPrefix_false.
-    + reflexivity.
-    + rewrite HeqH2.
-      reflexivity.
-  - repeat KRSimplifySound_crunch.
-    replace (KRExprDenote_RegInitT k1 = KRExprDenote_RegInitT (KRSimplify_RegInitT k)) with
-        (KRExprDenote_RegInitT (KRSimplify_RegInitT k) = KRExprDenote_RegInitT k1). reflexivity.
-    apply my_eq_refl.
-  - repeat KRSimplifySound_crunch.
-    replace (KRExprDenote_Rule k1 = KRExprDenote_Rule (KRSimplify_Rule k)) with
-        (KRExprDenote_Rule (KRSimplify_Rule k) = KRExprDenote_Rule k1). reflexivity.
-    apply my_eq_refl.
-  - repeat KRSimplifySound_crunch.
-    replace (KRExprDenote_DefMethT k1 = KRExprDenote_DefMethT (KRSimplify_DefMethT k)) with
-        (KRExprDenote_DefMethT (KRSimplify_DefMethT k) = KRExprDenote_DefMethT k1). reflexivity.
-    apply my_eq_refl.
-  - repeat KRSimplifySound_crunch.
-  - repeat KRSimplifySound_crunch.
-  - repeat KRSimplifySound_crunch.
-Qed.
+(************************************************************************************************************)
 
-Theorem KRSimplifySound_list_DefMethT: forall e,
-    KRExprDenote_list_DefMethT e = KRExprDenote_list_DefMethT (KRSimplify_list_DefMethT e).
+Scheme KRExpr_list_string_mut := Induction for KRExpr_list_string Sort Prop
+  with KRExpr_list_list_string_mut := Induction for KRExpr_list_list_string Sort Prop
+  with KRExpr_Prop_mut := Induction for KRExpr_Prop Sort Prop.
+
+Ltac KRSimplifySound_setup3 mut H H0 H1 :=
+  intros;
+  eapply (mut
+            (fun e : KRExpr_list_string => KRExprDenote_list_string (KRSimplify_list_string e) = KRExprDenote_list_string e)
+            (fun e : KRExpr_list_list_string => KRExprDenote_list_list_string (KRSimplify_list_list_string e) = KRExprDenote_list_list_string e)
+            (fun e : KRExpr_Prop => KRExprDenote_Prop (KRSimplify_Prop e) = KRExprDenote_Prop e)
+         );
+  try (intros);try(autorewrite with KRSimplify); try(autorewrite with KRSimplifyTopSound); try(simpl); try (rewrite H); try  (rewrite H0); try (rewrite H1); try(reflexivity);intros.
+
+(************************************************************************************************************)
+
+Theorem KRSimplifySound_list_string: forall e,
+    KRExprDenote_list_string (KRSimplify_list_string e) = KRExprDenote_list_string e.
 Proof.
-  KRSimplifySound_setup KRExpr_list_DefMethT_mut H H0 H1.
+  KRSimplifySound_setup3 KRExpr_list_string_mut H H0 H1; repeat KRSimplifySound_unit.
+  - repeat KRSimplifySound_crunch.
   repeat KRSimplifySound_unit.
   repeat KRSimplifySound_crunch.
   - repeat KRSimplifySound_crunch.
@@ -189,10 +86,10 @@ Proof.
   - repeat KRSimplifySound_crunch.
 Qed.
 
-Theorem KRSimplifySound_list_ModuleElt: forall e,
-    KRExprDenote_list_ModuleElt e = KRExprDenote_list_ModuleElt (KRSimplify_list_ModuleElt e).
+Theorem KRSimplifySound_list_list_string: forall e,
+    KRExprDenote_list_list_string e = KRExprDenote_list_list_string (KRSimplify_list_list_string e).
 Proof.
-  KRSimplifySound_setup KRExpr_list_ModuleElt_mut H H0 H1.
+  KRSimplifySound_setup KRExpr_list_list_string_mut H H0 H1.
   repeat KRSimplifySound_unit.
   repeat KRSimplifySound_crunch.
   - repeat KRSimplifySound_crunch.
@@ -250,3 +147,63 @@ Proof.
   - repeat KRSimplifySound_crunch.
 Qed.
 
+Theorem KRSimplifySound_Prop: forall e,
+    KRExprDenote_Prop e = KRExprDenote_Prop (KRSimplify_Prop e).
+Proof.
+  KRSimplifySound_setup KRExpr_Prop_mut H H0 H1.
+  repeat KRSimplifySound_unit.
+  repeat KRSimplifySound_crunch.
+  - repeat KRSimplifySound_crunch.
+  - repeat KRSimplifySound_crunch.
+  - repeat KRSimplifySound_crunch.
+  - repeat KRSimplifySound_crunch.
+  - repeat KRSimplifySound_crunch.
+  - repeat KRSimplifySound_crunch.
+  - repeat KRSimplifySound_crunch.
+  - repeat KRSimplifySound_crunch.
+  - repeat KRSimplifySound_crunch.
+  - repeat KRSimplifySound_crunch.
+  - repeat KRSimplifySound_crunch.
+  - repeat KRSimplifySound_crunch.
+  - repeat KRSimplifySound_crunch.
+  - repeat KRSimplifySound_crunch.
+  - repeat KRSimplifySound_crunch.
+  - repeat KRSimplifySound_crunch.
+  - repeat KRSimplifySound_crunch.
+  - repeat KRSimplifySound_crunch.
+  - repeat KRSimplifySound_crunch.
+  - repeat KRSimplifySound_crunch.
+  - repeat KRSimplifySound_crunch.
+  - repeat KRSimplifySound_crunch.
+  - repeat KRSimplifySound_crunch.
+  - repeat KRSimplifySound_crunch.
+  - repeat KRSimplifySound_crunch.
+  - repeat KRSimplifySound_crunch.
+  - repeat KRSimplifySound_crunch.
+  - repeat KRSimplifySound_crunch.
+  - repeat KRSimplifySound_crunch.
+  - repeat KRSimplifySound_crunch.
+    replace (KRExprDenote_string k1 = KRExprDenote_string (KRSimplify_string k)) with
+        (KRExprDenote_string (KRSimplify_string k) = KRExprDenote_string k1). reflexivity.
+    apply my_eq_refl.
+  - repeat KRSimplifySound_crunch.
+    erewrite sdisjPrefix_false.
+    + reflexivity.
+    + rewrite HeqH2.
+      reflexivity.
+  - repeat KRSimplifySound_crunch.
+    replace (KRExprDenote_RegInitT k1 = KRExprDenote_RegInitT (KRSimplify_RegInitT k)) with
+        (KRExprDenote_RegInitT (KRSimplify_RegInitT k) = KRExprDenote_RegInitT k1). reflexivity.
+    apply my_eq_refl.
+  - repeat KRSimplifySound_crunch.
+    replace (KRExprDenote_Rule k1 = KRExprDenote_Rule (KRSimplify_Rule k)) with
+        (KRExprDenote_Rule (KRSimplify_Rule k) = KRExprDenote_Rule k1). reflexivity.
+    apply my_eq_refl.
+  - repeat KRSimplifySound_crunch.
+    replace (KRExprDenote_DefMethT k1 = KRExprDenote_DefMethT (KRSimplify_DefMethT k)) with
+        (KRExprDenote_DefMethT (KRSimplify_DefMethT k) = KRExprDenote_DefMethT k1). reflexivity.
+    apply my_eq_refl.
+  - repeat KRSimplifySound_crunch.
+  - repeat KRSimplifySound_crunch.
+  - repeat KRSimplifySound_crunch.
+Qed.
