Rewrites/ReflectionSoundTopTheorems.v
@@ -11,7 +11,7 @@ Proof.
   solve_KRSimplifyTopSound.
 Qed.
 
-Hint Rewrite KRSimplifyTopSound_RegInitT : KRSimplifyTopSound.
+Hint Rewrite KRSimplifyTopSound_RegInitT : KRSimplify.
 
 Theorem KRSimplifyTopSound_Rule: forall e,
      KRExprDenote_Rule (KRSimplifyTop_Rule e)=KRExprDenote_Rule e.
@@ -19,7 +19,7 @@ Proof.
   solve_KRSimplifyTopSound.
 Qed.
 
-Hint Rewrite KRSimplifyTopSound_Rule : KRSimplifyTopSound.
+Hint Rewrite KRSimplifyTopSound_Rule : KRSimplify.
 
 Theorem KRSimplifyTopSound_DefMethT: forall e,
     KRExprDenote_DefMethT (KRSimplifyTop_DefMethT e)=KRExprDenote_DefMethT e.
@@ -27,7 +27,7 @@ Proof.
   solve_KRSimplifyTopSound.
 Qed.
 
-Hint Rewrite KRSimplifyTopSound_DefMethT : KRSimplifyTopSound.
+Hint Rewrite KRSimplifyTopSound_DefMethT : KRSimplify.
 
 Theorem KRSimplifyTopSound_ModuleElt: forall e,
     KRExprDenote_ModuleElt (KRSimplifyTop_ModuleElt e)=KRExprDenote_ModuleElt e.
@@ -35,16 +35,16 @@ Proof.
   solve_KRSimplifyTopSound.
 Qed.
 
-Hint Rewrite KRSimplifyTopSound_ModuleElt : KRSimplifyTopSound.
+Hint Rewrite KRSimplifyTopSound_ModuleElt : KRSimplify.
 
 Theorem KRSimplifyTopSound_list_RegInitT: forall e,
     KRExprDenote_list_RegInitT (KRSimplifyTop_list_RegInitT e)=KRExprDenote_list_RegInitT e.
 Proof.
   solve_KRSimplifyTopSound;solve_KRSimplifyTopSound;
-  repeat solve_contKRSimplifyTopSound.
+    repeat solve_contKRSimplifyTopSound.
 Qed.
 
-Hint Rewrite KRSimplifyTopSound_list_RegInitT : KRSimplifyTopSound.
+Hint Rewrite KRSimplifyTopSound_list_RegInitT : KRSimplify.
 
 Theorem KRSimplifyTopSound_list_list_RegInitT: forall e,
    KRExprDenote_list_list_RegInitT (KRSimplifyTop_list_list_RegInitT e)=KRExprDenote_list_list_RegInitT e.
@@ -53,7 +53,7 @@ Proof.
     repeat solve_contKRSimplifyTopSound.
 Qed.
 
-Hint Rewrite KRSimplifyTopSound_list_list_RegInitT : KRSimplifyTopSound.
+Hint Rewrite KRSimplifyTopSound_list_list_RegInitT : KRSimplify.
 
 Theorem KRSimplifyTopSound_list_Rule: forall e,
    KRExprDenote_list_Rule (KRSimplifyTop_list_Rule e)=KRExprDenote_list_Rule e.
@@ -62,7 +62,7 @@ Proof.
     repeat solve_contKRSimplifyTopSound.
 Qed.
 
-Hint Rewrite KRSimplifyTopSound_list_Rule : KRSimplifyTopSound.
+Hint Rewrite KRSimplifyTopSound_list_Rule : KRSimplify.
 
 Theorem KRSimplifyTopSound_list_list_Rule: forall e,
    KRExprDenote_list_list_Rule (KRSimplifyTop_list_list_Rule e)=KRExprDenote_list_list_Rule e.
@@ -71,7 +71,7 @@ Proof.
     repeat solve_contKRSimplifyTopSound.
 Qed.
 
-Hint Rewrite KRSimplifyTopSound_list_list_Rule : KRSimplifyTopSound.
+Hint Rewrite KRSimplifyTopSound_list_list_Rule : KRSimplify.
 
 Theorem KRSimplifyTopSound_list_DefMethT: forall e,
     KRExprDenote_list_DefMethT (KRSimplifyTop_list_DefMethT e)=KRExprDenote_list_DefMethT e.
@@ -80,7 +80,7 @@ Proof.
     repeat solve_contKRSimplifyTopSound.
 Qed.
 
-Hint Rewrite KRSimplifyTopSound_list_DefMethT : KRSimplifyTopSound.
+Hint Rewrite KRSimplifyTopSound_list_DefMethT : KRSimplify.
 
 Theorem KRSimplifyTopSound_list_ModuleElt: forall e,
     KRExprDenote_list_ModuleElt (KRSimplifyTop_list_ModuleElt e)=KRExprDenote_list_ModuleElt e.
@@ -90,7 +90,7 @@ Proof.
   repeat solve_contKRSimplifyTopSound.
 Qed.
 
-Hint Rewrite KRSimplifyTopSound_list_ModuleElt : KRSimplifyTopSound.
+Hint Rewrite KRSimplifyTopSound_list_ModuleElt : KRSimplify.
 
 Theorem KRSimplifyTopSound_list_list_ModuleElt: forall e,
     KRExprDenote_list_list_ModuleElt (KRSimplifyTop_list_list_ModuleElt e)=KRExprDenote_list_list_ModuleElt e.
@@ -100,7 +100,7 @@ Proof.
   repeat solve_contKRSimplifyTopSound.
 Qed.
 
-Hint Rewrite KRSimplifyTopSound_list_list_ModuleElt : KRSimplifyTopSound.
+Hint Rewrite KRSimplifyTopSound_list_list_ModuleElt : KRSimplify.
 
 Theorem KRSimplifyTopSound_string: forall e,
     KRExprDenote_string (KRSimplifyTop_string e)=KRExprDenote_string e.
@@ -109,7 +109,7 @@ Proof.
     repeat solve_contKRSimplifyTopSound.
 Qed.
 
-Hint Rewrite KRSimplifyTopSound_string : KRSimplifyTopSound.
+Hint Rewrite KRSimplifyTopSound_string : KRSimplify.
 
 Theorem KRSimplifyTopSound_list_string: forall e,
     KRExprDenote_list_string (KRSimplifyTop_list_string e)=KRExprDenote_list_string e.
@@ -119,7 +119,7 @@ Proof.
   repeat solve_contKRSimplifyTopSound.
 Qed.
 
-Hint Rewrite KRSimplifyTopSound_list_string : KRSimplifyTopSound.
+Hint Rewrite KRSimplifyTopSound_list_string : KRSimplify.
 
 Theorem KRSimplifyTopSound_list_list_string: forall e,
     KRExprDenote_list_list_string (KRSimplifyTop_list_list_string e)=KRExprDenote_list_list_string e.
@@ -129,7 +129,7 @@ Proof.
   repeat solve_contKRSimplifyTopSound.
 Qed.
 
-Hint Rewrite KRSimplifyTopSound_list_list_string : KRSimplifyTopSound.
+Hint Rewrite KRSimplifyTopSound_list_list_string : KRSimplify.
 
 Theorem KRSimplifyTopSound_BaseModule: forall e,
     KRExprDenote_BaseModule (KRSimplifyTop_BaseModule e)=KRExprDenote_BaseModule e.
@@ -139,7 +139,7 @@ Proof.
   repeat solve_contKRSimplifyTopSound.
 Qed.
 
-Hint Rewrite KRSimplifyTopSound_BaseModule : KRSimplifyTopSound.
+Hint Rewrite KRSimplifyTopSound_BaseModule : KRSimplify.
 
 Theorem KRSimplifyTopSound_Mod: forall e,
      KRExprDenote_Mod (KRSimplifyTop_Mod e)=KRExprDenote_Mod e.
@@ -149,7 +149,7 @@ Proof.
   repeat solve_contKRSimplifyTopSound.
 Qed.
 
-Hint Rewrite KRSimplifyTopSound_Mod : KRSimplifyTopSound.
+Hint Rewrite KRSimplifyTopSound_Mod : KRSimplify.
 
 Theorem KRSimplifyTopSound_list_Mod: forall e,
      KRExprDenote_list_Mod (KRSimplifyTop_list_Mod e)=KRExprDenote_list_Mod e.
@@ -159,7 +159,7 @@ Proof.
   repeat solve_contKRSimplifyTopSound.
 Qed.
 
-Hint Rewrite KRSimplifyTopSound_list_Mod : KRSimplifyTopSound.
+Hint Rewrite KRSimplifyTopSound_list_Mod : KRSimplify.
 
 Theorem KRSimplifyTopSound_RegFileBase: forall e,
      KRExprDenote_RegFileBase (KRSimplifyTop_RegFileBase e)=KRExprDenote_RegFileBase e.
@@ -169,7 +169,7 @@ Proof.
   repeat solve_contKRSimplifyTopSound.
 Qed.
 
-Hint Rewrite KRSimplifyTopSound_RegFileBase : KRSimplifyTopSound.
+Hint Rewrite KRSimplifyTopSound_RegFileBase : KRSimplify.
 
 Theorem KRSimplifyTopSound_list_RegFileBase: forall e,
      KRExprDenote_list_RegFileBase (KRSimplifyTop_list_RegFileBase e)=KRExprDenote_list_RegFileBase e.
@@ -179,7 +179,7 @@ Proof.
   repeat solve_contKRSimplifyTopSound.
 Qed.
 
-Hint Rewrite KRSimplifyTopSound_list_RegFileBase : KRSimplifyTopSound.
+Hint Rewrite KRSimplifyTopSound_list_RegFileBase : KRSimplify.
 
 Theorem KRSimplifyTopSound_Prop: forall e,
     KRExprDenote_Prop (KRSimplifyTop_Prop e)=KRExprDenote_Prop e.
@@ -204,5 +204,5 @@ Proof.
     apply my_eq_refl.
 Qed.
 
-Hint Rewrite KRSimplifyTopSound_Prop : KRSimplifyTopSound.
+Hint Rewrite KRSimplifyTopSound_Prop : KRSimplify.
 
